src/Dafny/util/marshal.i.dfy
@@ -109,6 +109,12 @@ function decode_uint64(bs: seq<byte>): (x:uint64)
     le_dec64(bs)
 }
 
+lemma decode_encode_uint64(x: uint64)
+    ensures decode_uint64(enc_encode(EncUInt64(x))) == x
+{
+    lemma_le_enc_dec64(x);
+}
+
 function decode_uint64_seq(bs: seq<byte>): (es: seq<uint64>)
     requires |bs| % 8 == 0
     ensures seq_encode(seq_fmap(encUInt64, es)) == bs
@@ -120,6 +126,18 @@ function decode_uint64_seq(bs: seq<byte>): (es: seq<uint64>)
         assert seq_fmap(encUInt64, es) == [EncUInt64(es[0])] + seq_fmap(encUInt64, es[1..]);
         es
     )
+}
+
+lemma decode_encode_uint64_seq_id(es: seq<uint64>)
+    ensures (enc_uint64_len(es);
+            decode_uint64_seq(seq_encode(seq_fmap(encUInt64, es))) == es)
+{
+    if es == [] { return; }
+    decode_encode_uint64(es[0]);
+    decode_encode_uint64_seq_id(es[1..]);
+    enc_uint64_len(es[1..]);
+    assert seq_fmap(encUInt64, es[1..]) == seq_fmap(encUInt64, es)[1..];
+    assert seq_encode(seq_fmap(encUInt64, es[1..])) == seq_encode(seq_fmap(encUInt64, es))[8..];
 }
 
 class Encoder
